Half of rewrite done

ulib/experimental/Steel.Extracted.ArrayStruct.fsti
@@ -23,7 +23,7 @@ module Map = FStar.Map
 
 
 open FStar.FunctionalExtensionality
-module PCM = Steel.PCM
+open Steel.PCM
 module UPCM = Steel.PCM.Unitless
 module UPCMBase = Steel.PCM.Unitless.Base
 module PCMBase = Steel.PCM.Base
@@ -32,130 +32,268 @@ open Steel.PCM.Effect
 open Steel.PCM.Memory
 
 /// This module defines a mechanism for extracting arraystructs compatible with separation logic
-/// into C arraystructs via Kremlin
+/// into C arraystructs via Kremlin. This is a rough sketch of Proposal 5 as described here
+/// https://github.com/FStarLang/FStar/wiki/Array-Structs-in-Steel
 
 #set-options "--fuel 0 --ifuel 0"
 
-(* foo is the view of what you're storing *)
-type foo : Type u#1 =
-  | MkFoo : x: UInt32.t -> y: UInt32.t -> z: UInt64.t -> foo
 
-(* low_foo is the low-level representation of [foo] *)
-type low_foo : Type u#1 = {
-  xy: Seq.lseq UInt32.t 2;
-  z: UInt64.t
+(*** The arraystruct typeclass *)
+
+/// The core of proposal 5 is to define a grammar of attributes for memory actions that Kremlin can
+/// recognize and extract as C arraystruct manipulation primitives. As such, these extractable memory
+/// actions should operate on types that represent C arraystructs, like Seq.lseq for arrays or F* structs for structs.
+
+/// However, we don't want to restrict the type manipulated by extractable Steel programs to just
+/// Seq.lseq or F* structs. To let the user freely work on user-defined, high-level types while
+/// maintaining a connection to low-level extractable types, we define a typeclass.
+
+(* Ongoing example: foo_view is the high-level view of what you're storing *)
+type foo_view : Type u#1 = {
+  view_x: UInt32.t;
+  view_y: UInt32.t;
+  view_z: UInt64.t
 }
-
-val foo_to_low_foo : foo -> low_foo
-
-(* The representation of the objects managed by [foo_pcm] in memory is low_foo *)
-(* [@@repr [low_foo, foo_to_low_foo, low_foo_to_foo]] *)
-val foo_pcm : PCM.pcm foo
-(* Suppose the [foo_pcm] mandates that z >= x + y *)
-
-class low_level_type (a: Type u#a) = {
-  pcm: PCM.pcm a;
-  low_a: Type u#a;
-  a_to_low_a: a -> low_a;
-}
-
-(* Check by tactic that [low_a] corresponds to something like Steel.PCM.ArrayStruct.descriptor *)
 
 (*
-  Second tactic : if [a] is already in the [low_a] format, then have a tactic that metaprograms
-  all the getters and setters.
-  Future work, only after we have a working setup
+  Ongoing example: foo_low is the low-level representation of [foo_view],
+  compatible with Kremlin extraction
 *)
-
-instance low_level_foo : low_level_type foo = {
-  pcm = foo_pcm;
-  low_a = low_foo;
-  a_to_low_a = foo_to_low_foo;
+type foo_low : Type u#1 = {
+  low_xy: Seq.lseq UInt32.t 2;
+  low_z: UInt64.t
 }
-
-open FStar.Tactics.Typeclasses
-
-(* Raise a GitHub issue for a typeclass syntax withing val signatures *)
-let ref (a: Type u#a) (#[tcresolve ()] ca:low_level_type a) : Type u#0  = ref a ca.pcm
-
-let ref_hprop (#a: Type u#a) (#[tcresolve ()] ca:low_level_type a) (r: ref a) : slprop u#a =
-  h_exists (pts_to r)
-
-(* Buggy, use selectors here*)
-val sel (#a: Type) (#[tcresolve ()] ca:low_level_type a) (r: ref a) (h: hmem (ref_hprop r))  : GTot a
-
-#set-options "--print_implicits --print_universes --z3rlimit 20 --prn"
-
-val alloc
-  (#a: Type u#1) (#[FStar.Tactics.Typeclasses.tcresolve ()] ca: low_level_type a)
-  (v: a) (#[FStar.Tactics.exact (quote (ca.a_to_low_a v))] v_low: ca.low_a)
-    : Steel (ref a #ca) emp (fun r -> ref_hprop r) (fun _ -> True) (fun _ r h1 -> (* sel h1 r == v*) True)
-
-let main () =
-  alloc #foo (MkFoo 0ul 0ul 1UL)
-
-
-(* You have to give update_z because you have to justify this with regards to [foo_pcm] *)
-
-
-val update: unit -> Tot unit
-val get: unit -> Tot unit
-val focus: unit -> Tot unit
-val explode: unit -> Tot unit
-val op_String_Access : unit -> Tot unit
 
 open FStar.Tactics
 
-let check (src: string) : Tac unit =
-  let _ = lookup_typ (top_env ()) (cur_module () @ [ src ]) in
+(**
+  This tactics checks whether a declared type falls into the subset allowed by Kremlin.
+  Can also be done at extraction but less useful error messages
+*)
+let check_low (src: string) : Tac unit =
   exact (`(()))
 
-(* What checks for this attribute ?
-    - number of arguments: 2
-    - first argument is ref to type that has low_level_type typeclass
-    - [low_foo] is [low_a] for that typeclass
-    - z is a field of low_foo (low_foo has to be a record)
-    - postcondition implies that (a_to_low_a (sel h1 r))  == { a_to_low_a (sel h0 r) with z = new_val }
-  *)
-[@@ update low_foo.z]
-val update_z (r: ref foo) (new_val: UInt64.t)
-    : Steel unit (ref_hprop r) (fun _ -> ref_hprop r) (
-      let pre : hmem (ref_hprop r) -> prop = fun h0 ->
-        if UInt64.v new_val >= UInt32.v (sel r h0).x + UInt32.v (sel r h0).y then
-          True else False
-      in
-      assume(respects_fp pre);
-      pre
-    ) (
-      let post : hmem (ref_hprop r) -> unit -> hmem (ref_hprop r) -> prop  =
-        fun h0 _ h1 -> (sel r h1) == MkFoo (sel r h0).x (sel r h0).y new_val
-      in
-      assume(respects_binary_fp post);
-      post
-    )
+(* Ongoing example : this check could be inserted via some metaprogramming or surface language *)
+let _ : unit  = _ by (check_low (`%foo_low))
 
-let _ : unit  = _ by (check (`%update_z))
+/// Now to finish relating the view and the low-level representation, we need a bijection.
 
-(* What does this attribute check ?
-    - number of arguments: 2
-    - first argument is ref to type that has low_level_type typeclass
-    - [low_foo] is [low_a] for that typeclass
-    - .x.[0] is a subpath of low_foo
-    - postcondition (fun h0 x h1) implies that (
-      a_to_low_a (sel h0 r) == a_to_low_a (sel h1 r) /\
-      x == a_to_low_a (sel h1 r).x.[0]
-     )
+(* Ongoing example: bijection between [foo_low] and [foo_view] *)
+let foo_low_to_view (l: foo_low) : foo_view = {
+  view_x = Seq.index l.low_xy 0;
+  view_y = Seq.index l.low_xy 1;
+  view_z = l.low_z;
+}
+let foo_view_to_low (v: foo_view) : foo_low = {
+  low_xy = Seq.init 2 (fun i -> if i = 0 then v.view_x else v.view_y);
+  low_z = v.view_z
+}
+
+
+(**
+  This typeclass contains all the informations the extraction grammar needs to extract view
+  manipulations into low-level C primitives
 *)
+class low_level (view: Type u#a) = {
+  low: Type u#a;
+  view_to_low: view -> low;
+  low_to_view: low -> view;
+  bijection_one: (x: view) -> Lemma (low_to_view (view_to_low x) == x);
+  bijection_two: (x: low) -> Lemma (view_to_low (low_to_view x) == x)
+}
 
-[@@get low_foo.x.[0]]
-val get_x (r: ref foo)
-  : Steel UInt32.t (ref_hprop r) (fun _ -> ref_hprop r) (fun _ -> True) (
-    let post : hmem (ref_hprop r) -> UInt32.t -> hmem (ref_hprop r) -> prop =
-      fun h0 x h1 -> (sel r h0 == sel r h1 /\ x == (sel r h1).x)
-    in
-    assume(respects_binary_fp post);
-    post
+(* Ongoing example: this is the [foo] instance of the type class *)
+instance low_level_foo : low_level foo_view = {
+  low = foo_low;
+  view_to_low = foo_view_to_low;
+  low_to_view = foo_low_to_view;
+  bijection_one = (fun _ -> ());
+  bijection_two = (fun l ->
+    let new_l = foo_view_to_low (foo_low_to_view l) in
+    assert(new_l.low_xy `Seq.equal` l.low_xy)
   )
+}
+
+/// Please note that if you are working with types that are already extractable by Kremlin, then
+/// it is trivial to implement that typeclass by taking everything as identity. The typeclass
+/// implementation can then be metaprogrammed.
+
+(*** The attribute grammar in actions *)
+
+/// Let us now illustrate what the attribute language will look like by annotating memory actions,
+/// either generic for all low/view pairs or on our ongoing example [foo].
+
+open FStar.Tactics.Typeclasses
+
+(** We are going to use pre/post conditions for specifications in Steel, so we need this helper *)
+let slref (#a: Type u#a) (#pcm: pcm a) (r: ref a pcm) : slprop u#a =
+  h_exists (pts_to r)
+
+(**
+  Also this helper [sel] function will allow use to retrieve the values of references witout
+  while we don't have selectors.
+*)
+val sel (#a: Type) (#pcm: pcm a) (r: ref a pcm) (h: hmem (slref r)) : GTot a
+
+(** We pretend we have a PCM for the view of [foo] *)
+val foo_pcm : pcm foo_view
+
+(** We don't bother proving the self-framedness of pre/postconditions in this sketch *)
+val admitted_post
+  (#a: Type) (#pre:slprop) (#post: a -> slprop)
+  (p:(hmem pre -> x:a -> hmem (post x) -> prop))
+  : GTot (p:(hmem pre -> x:a -> hmem (post x) -> prop){respects_binary_fp p})
+
+val admitted_pre
+  (#pre:slprop)
+  (p:(hmem pre -> prop))
+  : GTot (p:(hmem pre -> prop){respects_fp p})
+
+/// To ensure that the attribute grammar typechecks, we have to define dummy functions so that
+/// the names are recognized.
+
+val extract_update: unit -> Tot unit
+val extract_get: unit -> Tot unit
+val extract_focus: unit -> Tot unit
+val extract_explode: unit -> Tot unit
+val op_String_Access : unit -> Tot unit
+val generic_index: unit -> Tot unit
+
+(**** alloc *)
+
+/// The alloc action can be specified generically to all view/low type pairs, no need for an
+/// attribute here.
+
+val alloc
+  (#a: Type u#1)
+  (#[FStar.Tactics.Typeclasses.tcresolve ()] ca: low_level a)
+  (pcm: pcm a)
+  (v: a)
+  (#[FStar.Tactics.exact (quote (ca.view_to_low v))] v_low: ca.low)
+    : Steel (ref a pcm) emp (fun r -> slref r) (fun _ -> True) (admitted_post (fun _ r h1 -> sel r h1 == v))
+
+(**** update *)
+
+/// The update operation is more complicated, since the way you can update your view depend on the
+/// PCM that is attached to it. This is where the attribute grammar for extraction is going to be
+/// useful. Let us say that [foo_pcm] requires us to maintain the following invariant:
+/// ```
+/// f.view_x + f.view_y <= f.view_z
+/// ```
+/// Let us also suppose that we want to update the [z] field of the object, then the action should
+/// take the whole object in order to ensure the invariant is respected. However, we only want
+/// this update to be extracted to an update of the [z] field in C. This is how we would write it:
+
+[@@ extract_update foo_low.low_z]
+val update_z (r: ref foo_view foo_pcm) (new_val: UInt64.t)
+    : Steel unit (slref r) (fun _ -> slref r)
+    (admitted_pre (fun h0 -> (* Question : why do we need the if here? Universes? *)
+      if UInt64.v new_val >= UInt32.v (sel r h0).view_x + UInt32.v (sel r h0).view_y then
+        True else False
+    )) (admitted_post (fun h0 _ h1 ->
+     (sel r h1) == { sel r h0 with view_z = new_val }
+    ))
+
+/// What should the attribute `[@@extract_update foo_low.low_z]` check for the signature of
+/// `update_z` ?
+///  - `extract_update` means that `update_z` should have two arguments, the first being the
+///     reference and the second being the new value
+///  - `low_foo` means that the reference should point to a type for which `low_foo` is an instance
+///     of the `low_level` typeclass
+///  - `low_z` can actually be a path into the low-level structs, a sequence of field accesses and
+///     array indexes. The type of the new value for update should correspond to the low-level type
+///     at the end of the path in the low-level structure
+///  -  pre and post-ressource should be `slref r`, return type unit
+///  -  finally, the postcondition of `update_z` should imply the following semantic definition
+///     of a low-level update:
+///     ```
+///     foo_view_to_low (sel h1 r) == { foo_view_to_low (sel h0 r) with z = new_val }
+///     ```
+///
+/// While the first 4 checks are completely syntactic, the last one can be discharged to SMT. Please
+/// note that the bijection is important here because it will allow us to prove this last semantic
+/// obligation, by "lifting" the equality in the low-level world to the high-level views where
+/// the real postcondition of the function is specified.
+
+(* Ongoing example: sketch on how to use a tactic for checking what is described above *)
+let check_extract_update (src: string) : Tac unit =
+  exact (`(()))
+
+let _ : unit  = _ by (check_extract_update (`%update_z))
+
+/// Some comments about the meta-arguments that justify the soundness of extraction, given an
+/// update with attribute that respect all of the above conditions.
+///
+/// We now thanks to separation logic that `update_z` can only modify the memory location of
+/// reference [r], and nothing else.
+/// This meta-argument justifies the fact that it is admissible to compile `update_z` with a mere
+/// memory update. `update_z` can do other things such as allocating a new address and then ditching
+/// it, but this is not observable by another thread in our semantic. So we eliminate by extracting
+/// to Kremlin execution traces that are unobservable and didn't change the computation result.
+///
+/// What if [update_z] assigns first one value then another? Then we claim that it does not matter since this more complicated execution trace will be extracted by Kremlin to a simpler one. In F*
+/// you would still have to prove that the F* body of `update_z` is frame perserving, so if you do
+/// that then the frame preservedness still holds for the simpler version extracted by Kremlin.
+///
+/// The bijection is also key for our meta-argument here. Let's imagine in the low version we have
+/// an additional field that is useless, i.e. it is not mapped to a view filed. Because of the
+/// bijection between the view and the low-level type, then the value of the useless field has to be
+/// constant; otherwise you couldn't prove the bijection.
+/// So your update function  could write anything that it wants on that useless field, but it's
+/// generally forbidden because the useless field needs to have always the same value. You could write
+/// the same value into it but that would fall under redundant write elimination.
+
+(**** get *)
+
+/// Let us now see what how to annotate a function corresponding to a low-level read.
+
+[@@extract_get foo_low.low_xy.[0]]
+val get_x (r: ref foo_view foo_pcm)
+  : Steel UInt32.t
+  (slref r) (fun _ -> slref r)
+  (fun _ -> True) (admitted_post (fun h0 v h1 ->
+    sel r h0 == sel r h1 /\ v == (sel r h1).view_x
+  ))
+
+/// The attribute `[@@extract_get foo_low.low_xy.[0]]` still has to check syntactically that the
+/// signature of `get_x` corresponds to a low-level get (one argument which is a ref, returns
+/// a value of the right type).
+///
+/// You can see here that the inner path that we use is more complex (`.low_xy.[0]`). So what is the
+/// semantic post-condition implication check here ? Let's call `v` the returned value
+///
+/// ```
+///   foo_view_to_low (sel h0 r) == foo_view_to_low (sel h1 r) /\
+///   v == foo_view_to_low (sel h1 r).x.[0]
+/// ```
+///
+
+(**** low-level array indexing *)
+
+/// The last example updates an array cell with a constant index, but let's see what a get function
+/// working on a generic index would look like.
+
+[@@extract_get foo_low.low_xy.[generic_index]]
+val get_xy_i (r: ref foo_view foo_pcm) (i: SizeT.t)
+  : Steel UInt32.t
+  (slref r) (fun _ -> slref r)
+  (admitted_pre (fun _ -> if SizeT.v i < 2 then True else False)) (admitted_post (fun h0 ret h1 ->
+    sel r h0 == sel r h1 /\ (
+      if SizeT.v i = 0 then
+        ret == (sel r h1).view_x
+      else if SizeT.v i = 1 then
+        ret == (sel r h1).view_y
+      else False
+  )))
+
+/// On top of the syntactic checks, the attribute should check that the precondition implies that the
+/// index argument is withing the bounds of the low-level array. The postcondition should imply that,
+/// if v is the returned value,
+///
+/// ```
+///  foo_view_to_low (sel r h1) == foo_view_to_low (sel r h1) /\
+///  v == Seq.index (foo_view_to_low (sel r h1)).low_xy i
+/// ```
 
 (* Language of attributes :
    [@@ update low_struct.field]
@@ -240,13 +378,12 @@ let foo_to_xy_z (x: foo)
     - number of arguments: 1
     - first argument is ref to type that has low_level_type typeclass
     - [low_foo] is [low_a] for that typeclass
-    - possibly check for a path of low_foo
     - return type is tupleof refs to the right typeclasses
     - postcondition implies
        a_to_low_a (sel h0 r) == a_to_low_a (sel h1 r) /\
        (sel h1 r1', sel h1 r2') == foo_to_xy_z (sel h0 r)
 *)
-[@@explode low_foo -> (low_level_xy, low_level_z) -> foo_to_xy_z]
+[@@explode low_foo -> foo_to_xy_z -> (low_level_xy, low_level_z) ]
 val explode_xy_z (r: ref foo)
   : Steel (
     ref (Seq.lseq (Universe.raise_t UInt32.t) 2) #low_level_xy &
